
module Oscar.Data.Substitunction {𝔣} (FunctionName : Set 𝔣) where

open import Oscar.Data.Equality
open import Oscar.Data.Equality.properties
open import Oscar.Data.Fin
open import Oscar.Data.Nat
open import Oscar.Data.Term FunctionName
open import Oscar.Data.Vec
open import Oscar.Function
open import Oscar.Level
open import Oscar.Relation

-- Substitunction
_⊸_ : (m n : Nat) → Set 𝔣
m ⊸ n = Fin m → Term n

▸ : ∀ {m n} → m ⟨ Fin ⟩→ n → m ⊸ n
▸ r = i ∘ r

infix 19 _◂_ _◂s_

mutual

  _◂_ : ∀ {m n} → m ⊸ n → m ⟨ Term ⟩→ n
  σ̇ ◂ i 𝑥 = σ̇ 𝑥
  _ ◂ leaf = leaf
  σ̇ ◂ (τl fork τr) = (σ̇ ◂ τl) fork (σ̇ ◂ τr)
  σ̇ ◂ (function fn τs) = function fn (σ̇ ◂s τs) where

  _◂s_ : ∀ {m n} → m ⊸ n → ∀ {N} → m ⟨ Terms N ⟩→ n  -- Vec (Term m) N → Vec (Term n) N
  f ◂s [] = []
  f ◂s (t ∷ ts) = f ◂ t ∷ f ◂s ts

_∙_ : ∀ {m n} → m ⊸ n → ∀ {l} → l ⊸ m → l ⊸ n
_∙_ f g = (f ◂_) ∘ g

mutual

  ◂-extensionality : ∀ {m n} {f g : m ⊸ n} → f ≡̇ g → f ◂_ ≡̇ g ◂_
  ◂-extensionality p (i x) = p x
  ◂-extensionality p leaf = refl
  ◂-extensionality p (s fork t) = cong₂ _fork_ (◂-extensionality p s) (◂-extensionality p t)
  ◂-extensionality p (function fn ts) = cong (function fn) (◂s-extensionality p ts)

  ◂s-extensionality : ∀ {m n} {f g : m ⊸ n} → f ≡̇ g → ∀ {N} → _◂s_ f {N} ≡̇ _◂s_ g
  ◂s-extensionality p [] = refl
  ◂s-extensionality p (t ∷ ts) = cong₂ _∷_ (◂-extensionality p t) (◂s-extensionality p ts)

mutual

  ◂-associativity : ∀ {l m} (f : l ⊸ m) {n} (g : m ⊸ n) → (g ∙ f) ◂_ ≡̇ (g ◂_) ∘ (f ◂_)
  ◂-associativity _ _ (i _) = refl
  ◂-associativity _ _ leaf = refl
  ◂-associativity _ _ (τ₁ fork τ₂) = cong₂ _fork_ (◂-associativity _ _ τ₁) (◂-associativity _ _ τ₂)
  ◂-associativity f g (function fn ts) = cong (function fn) (◂s-associativity f g ts)

  ◂s-associativity : ∀ {l m n} (f : l ⊸ m) (g : m ⊸ n) → ∀ {N} → (_◂s_ (g ∙ f) {N}) ≡̇ (g ◂s_) ∘ (f ◂s_)
  ◂s-associativity _ _ [] = refl
  ◂s-associativity _ _ (τ ∷ τs) = cong₂ _∷_ (◂-associativity _ _ τ) (◂s-associativity _ _ τs)

∙-associativity : ∀ {k l} (f : k ⊸ l) {m} (g : l ⊸ m) {n} (h : m ⊸ n) → (h ∙ g) ∙ f ≡̇ h ∙ (g ∙ f)
∙-associativity f g h x rewrite ◂-associativity g h (f x) = refl

∙-extensionality : ∀ {l m} {f₁ f₂ : l ⊸ m} → f₁ ≡̇ f₂ → ∀ {n} {g₁ g₂ : m ⊸ n} → g₁ ≡̇ g₂ → g₁ ∙ f₁ ≡̇ g₂ ∙ f₂
∙-extensionality {f₂ = f₂} f₁≡̇f₂ g₁≡̇g₂ x rewrite f₁≡̇f₂ x = ◂-extensionality g₁≡̇g₂ (f₂ x)

ε : ∀ {m} → m ⊸ m
ε = i

mutual

  ◂-identity : ∀ {m} (t : Term m) → ε ◂ t ≡ t
  ◂-identity (i x) = refl
  ◂-identity leaf = refl
  ◂-identity (s fork t) = cong₂ _fork_ (◂-identity s) (◂-identity t)
  ◂-identity (function fn ts) = cong (function fn) (◂s-identity ts)

  ◂s-identity : ∀ {N m} (t : Vec (Term m) N) → ε ◂s t ≡ t
  ◂s-identity [] = refl
  ◂s-identity (t ∷ ts) = cong₂ _∷_ (◂-identity t) (◂s-identity ts)

∙-left-identity : ∀ {m n} (f : m ⊸ n) → ε ∙ f ≡̇ f
∙-left-identity f = ◂-identity ∘ f

∙-right-identity : ∀ {m n} (f : m ⊸ n) → f ∙ ε ≡̇ f
∙-right-identity _ _ = refl

open import Oscar.Category

semigroupoidSubstitunction : Semigroupoid _⊸_ (λ {m n} → ≡̇-setoid (λ _ → Term n))
Semigroupoid._∙_ semigroupoidSubstitunction = _∙_
Semigroupoid.∙-extensionality semigroupoidSubstitunction = ∙-extensionality
Semigroupoid.∙-associativity semigroupoidSubstitunction = ∙-associativity

semigroupoidExtensionTerm : Semigroupoid (_⟨ Term ⟩→_) (λ {m n} → ≡̇-setoid (λ _ → Term n))
Semigroupoid._∙_ semigroupoidExtensionTerm g = g ∘_
Semigroupoid.∙-extensionality semigroupoidExtensionTerm {f₂ = f₂} f₁≡̇f₂ g₁≡̇g₂ x rewrite f₁≡̇f₂ x = g₁≡̇g₂ (f₂ x)
Semigroupoid.∙-associativity semigroupoidExtensionTerm _ _ _ _ = refl

semigroupoidExtensionTerms : ∀ N → Semigroupoid (_⟨ Terms N ⟩→_) (λ {m n} → ≡̇-setoid (λ _ → Terms N n))
Semigroupoid._∙_ (semigroupoidExtensionTerms _) g = g ∘_
Semigroupoid.∙-extensionality (semigroupoidExtensionTerms _) {f₂ = f₂} f₁≡̇f₂ g₁≡̇g₂ x rewrite f₁≡̇f₂ x = g₁≡̇g₂ (f₂ x)
Semigroupoid.∙-associativity (semigroupoidExtensionTerms _) _ _ _ _ = refl

semifunctorSubstitute : Semifunctor semigroupoidSubstitunction semigroupoidExtensionTerm
Semifunctor.μ semifunctorSubstitute = id
Semifunctor.𝔣 semifunctorSubstitute = _◂_
Semifunctor.𝔣-extensionality semifunctorSubstitute = ◂-extensionality
Semifunctor.𝔣-commutativity semifunctorSubstitute {f = f} {g = g} = ◂-associativity f g

semifunctorSubstitutes : ∀ N → Semifunctor semigroupoidSubstitunction (semigroupoidExtensionTerms N)
Semifunctor.μ (semifunctorSubstitutes _) = id
Semifunctor.𝔣 (semifunctorSubstitutes N) f τs = f ◂s τs
Semifunctor.𝔣-extensionality (semifunctorSubstitutes _) f≡̇g = ◂s-extensionality f≡̇g
Semifunctor.𝔣-commutativity (semifunctorSubstitutes _) {f = f} {g = g} = ◂s-associativity f g





------------ subfact3 : ∀ {l m n} (f : m ⊸ n) (r : l ⟨ Fin ⟩→ m) → f ◇ (▸ r) ≡ f ∘ r
------------ subfact3 f r = refl

-- -- -- -- prop-id : ∀ {m n} {f : _ ⊸ n} {ℓ} {P : ⊸-ExtentionalProperty {ℓ} m} → proj₁ P f → proj₁ P (i ◇ f)
-- -- -- -- prop-id {_} {_} {f} {_} {P'} Pf = proj₂ P' (λ x → sym (◃-identity (f x))) Pf

-- -- -- -- ≐-cong : ∀ {m n o} {f : m ⊸ n} {g} (h : _ ⊸ o) → f ≐ g → (h ◇ f) ≐ (h ◇ g)
-- -- -- -- ≐-cong h f≐g t = cong (h ◃_) (f≐g t)

-- -- -- -- -- data AList : ℕ -> ℕ -> Set 𝔣 where
-- -- -- -- --   anil : ∀ {n} -> AList n n
-- -- -- -- --   _asnoc_/_ : ∀ {m n} (σ : AList m n) (t' : Term m) (x : Fin (suc m))
-- -- -- -- --                -> AList (suc m) n

-- -- -- -- -- sub : ∀ {m n} (σ : AList m n) -> Fin m -> Term n
-- -- -- -- -- sub anil = i
-- -- -- -- -- sub (σ asnoc t' / x) = sub σ ◇ (t' for x)

-- -- -- -- -- _++_ : ∀ {l m n} (ρ : AList m n) (σ : AList l m) -> AList l n
-- -- -- -- -- ρ ++ anil = ρ
-- -- -- -- -- ρ ++ (σ asnoc t' / x) = (ρ ++ σ) asnoc t' / x

-- -- -- -- -- ++-assoc : ∀ {l m n o} (ρ : AList l m) (σ : AList n _) (τ : AList o _) -> ρ ++ (σ ++ τ) ≡ (ρ ++ σ) ++ τ
-- -- -- -- -- ++-assoc ρ σ anil = refl
-- -- -- -- -- ++-assoc ρ σ (τ asnoc t / x) = cong (λ s -> s asnoc t / x) (++-assoc ρ σ τ)

-- -- -- -- -- module SubList where
-- -- -- -- --   anil-id-l : ∀ {m n} (σ : AList m n) -> anil ++ σ ≡ σ
-- -- -- -- --   anil-id-l anil = refl
-- -- -- -- --   anil-id-l (σ asnoc t' / x) = cong (λ σ -> σ asnoc t' / x) (anil-id-l σ)

-- -- -- -- --   fact1 : ∀ {l m n} (ρ : AList m n) (σ : AList l m) -> sub (ρ ++ σ) ≐ (sub ρ ◇ sub σ)
-- -- -- -- --   fact1 ρ anil v = refl
-- -- -- -- --   fact1 {suc l} {m} {n} r (s asnoc t' / x) v = trans hyp-on-terms ◃-assoc
-- -- -- -- --     where
-- -- -- -- --       t = (t' for x) v
-- -- -- -- --       hyp-on-terms = ◃-extentionality (fact1 r s) t
-- -- -- -- --       ◃-assoc = ◃-associativity t

-- -- -- -- -- _∃asnoc_/_ : ∀ {m} (a : ∃ (AList m)) (t' : Term m) (x : Fin (suc m))
-- -- -- -- --   -> ∃ (AList (suc m))
-- -- -- -- -- (n , σ) ∃asnoc t' / x = n , σ asnoc t' / x

-- -- -- -- -- open import Data.Maybe using (Maybe; nothing; just)

-- -- -- -- -- flexFlex : ∀ {m} (x y : Fin m) -> ∃ (AList m)
-- -- -- -- -- flexFlex {suc m} x y with check x y
-- -- -- -- -- ...              | just y' = m , anil asnoc i y' / x
-- -- -- -- -- ...              | nothing = suc m , anil
-- -- -- -- -- flexFlex {zero} () _

-- -- -- -- -- open import Oscar.Class.ThickAndThin

-- -- -- -- -- flexRigid : ∀ {m} (x : Fin m) (t : Term m) -> Maybe (∃(AList m))
-- -- -- -- -- flexRigid {suc m} x t with check x t
-- -- -- -- -- ...                   | just t' = just (m , anil asnoc t' / x)
-- -- -- -- -- ...                   | nothing = nothing
-- -- -- -- -- flexRigid {zero} () _

-- -- -- -- -- -- open import Oscar.Data.Fin using (Fin; zero; suc; thick?; Check; check; thin; module Thick)

-- -- -- -- -- -- open import Data.Fin using (Fin; suc; zero)
-- -- -- -- -- -- open import Data.Nat hiding (_≤_)
-- -- -- -- -- -- open import Relation.Binary.PropositionalEquality renaming ([_] to [[_]])
-- -- -- -- -- -- open import Function using (_∘_; id; case_of_; _$_; flip)
-- -- -- -- -- -- open import Relation.Nullary
-- -- -- -- -- -- open import Data.Product renaming (map to _***_)
-- -- -- -- -- -- open import Data.Empty
-- -- -- -- -- -- open import Data.Maybe
-- -- -- -- -- -- open import Category.Functor
-- -- -- -- -- -- open import Category.Monad
-- -- -- -- -- -- import Level
-- -- -- -- -- -- open RawMonad (Data.Maybe.monad {Level.zero})
-- -- -- -- -- -- open import Data.Sum
-- -- -- -- -- -- open import Data.Maybe using (maybe; maybe′; nothing; just; monad; Maybe)
-- -- -- -- -- -- open import Data.List renaming (_++_ to _++L_)
-- -- -- -- -- -- open ≡-Reasoning
-- -- -- -- -- -- open import Data.Vec using (Vec; []; _∷_) renaming (_++_ to _++V_; map to mapV)

-- -- -- -- -- -- open import Data.Nat using (ℕ; suc; zero)
-- -- -- -- -- -- open import Relation.Binary.PropositionalEquality using (_≡_; refl; cong₂; cong; sym; trans)
-- -- -- -- -- -- open import Function using (_∘_; flip)
-- -- -- -- -- -- open import Relation.Nullary using (¬_; Dec; yes; no)
-- -- -- -- -- -- open import Data.Product using (∃; _,_; _×_)
-- -- -- -- -- -- open import Data.Empty using (⊥-elim)
-- -- -- -- -- -- open import Data.Vec using (Vec; []; _∷_)

-- -- -- -- -- -- Term-function-inj-FunctionName : ∀ {fn₁ fn₂} {n N₁ N₂} {ts₁ : Vec (Term n) N₁} {ts₂ : Vec (Term n) N₂} → Term.function fn₁ ts₁ ≡ Term.function fn₂ ts₂ → fn₁ ≡ fn₂
-- -- -- -- -- -- Term-function-inj-FunctionName refl = refl

-- -- -- -- -- -- Term-function-inj-VecSize : ∀ {fn₁ fn₂} {n N₁ N₂} {ts₁ : Vec (Term n) N₁} {ts₂ : Vec (Term n) N₂} → Term.function fn₁ ts₁ ≡ Term.function fn₂ ts₂ → N₁ ≡ N₂
-- -- -- -- -- -- Term-function-inj-VecSize refl = refl

-- -- -- -- -- -- Term-function-inj-Vector : ∀ {fn₁ fn₂} {n N} {ts₁ : Vec (Term n) N} {ts₂ : Vec (Term n) N} → Term.function fn₁ ts₁ ≡ Term.function fn₂ ts₂ → ts₁ ≡ ts₂
-- -- -- -- -- -- Term-function-inj-Vector refl = refl

-- -- -- -- -- -- Term-fork-inj-left : ∀ {n} {l₁ r₁ l₂ r₂ : Term n} → l₁ fork r₁ ≡ l₂ fork r₂ → l₁ ≡ l₂
-- -- -- -- -- -- Term-fork-inj-left refl = refl

-- -- -- -- -- -- Term-fork-inj-right : ∀ {n} {l₁ r₁ l₂ r₂ : Term n} → l₁ fork r₁ ≡ l₂ fork r₂ → r₁ ≡ r₂
-- -- -- -- -- -- Term-fork-inj-right refl = refl

-- -- -- -- -- -- open import Relation.Binary.HeterogeneousEquality using (_≅_; refl)

-- -- -- -- -- -- Term-function-inj-HetVector : ∀ {fn₁ fn₂} {n N₁ N₂} {ts₁ : Vec (Term n) N₁} {ts₂ : Vec (Term n) N₂} → Term.function fn₁ ts₁ ≡ Term.function fn₂ ts₂ → ts₁ ≅ ts₂
-- -- -- -- -- -- Term-function-inj-HetVector refl = refl

-- -- -- -- -- -- _⊸_ : (m n : ℕ) → Set
-- -- -- -- -- -- m ⊸ n = Fin m → Term n

-- -- -- -- -- -- ▸ : ∀ {m n} → (r : Fin m → Fin n) → Fin m → Term n
-- -- -- -- -- -- ▸ r = i ∘ r

-- -- -- -- -- -- record Substitution (T : ℕ → Set) : Set where
-- -- -- -- -- --   field
-- -- -- -- -- --     _◃_ : ∀ {m n} → (f : m ⊸ n) → T m → T n

-- -- -- -- -- -- open Substitution ⦃ … ⦄ public

-- -- -- -- -- -- {-# DISPLAY Substitution._◃_ _ = _◃_ #-}

-- -- -- -- -- -- mutual

-- -- -- -- -- --   instance SubstitutionTerm : Substitution Term
-- -- -- -- -- --   Substitution._◃_ SubstitutionTerm = _◃′_ where
-- -- -- -- -- --     _◃′_ : ∀ {m n} → (f : m ⊸ n) → Term m → Term n
-- -- -- -- -- --     f ◃′ i x = f x
-- -- -- -- -- --     f ◃′ leaf = leaf
-- -- -- -- -- --     f ◃′ (s fork t) = (f ◃ s) fork (f ◃ t)
-- -- -- -- -- --     f ◃′ (function fn ts) = function fn (f ◃ ts)

-- -- -- -- -- --   instance SubstitutionVecTerm : ∀ {N} → Substitution (flip Vec N ∘ Term )
-- -- -- -- -- --   Substitution._◃_ (SubstitutionVecTerm {N}) = _◃′_ where
-- -- -- -- -- --     _◃′_ : ∀ {m n} → (f : m ⊸ n) → Vec (Term m) N → Vec (Term n) N
-- -- -- -- -- --     f ◃′ [] = []
-- -- -- -- -- --     f ◃′ (t ∷ ts) = f ◃ t ∷ f ◃ ts

-- -- -- -- -- -- _≐_ : {m n : ℕ} → (Fin m → Term n) → (Fin m → Term n) → Set
-- -- -- -- -- -- f ≐ g = ∀ x → f x ≡ g x

-- -- -- -- -- -- record SubstitutionExtensionality (T : ℕ → Set) ⦃ _ : Substitution T ⦄ : Set₁ where
-- -- -- -- -- --   field
-- -- -- -- -- --     ◃ext : ∀ {m n} {f g : Fin m → Term n} → f ≐ g → (t : T m) → f ◃ t ≡ g ◃ t

-- -- -- -- -- -- open SubstitutionExtensionality ⦃ … ⦄ public

-- -- -- -- -- -- mutual

-- -- -- -- -- --   instance SubstitutionExtensionalityTerm : SubstitutionExtensionality Term
-- -- -- -- -- --   SubstitutionExtensionality.◃ext SubstitutionExtensionalityTerm = ◃ext′ where
-- -- -- -- -- --     ◃ext′ : ∀ {m n} {f g : Fin m → Term n} → f ≐ g → ∀ t → f ◃ t ≡ g ◃ t
-- -- -- -- -- --     ◃ext′ p (i x) = p x
-- -- -- -- -- --     ◃ext′ p leaf = refl
-- -- -- -- -- --     ◃ext′ p (s fork t) = cong₂ _fork_ (◃ext p s) (◃ext p t)
-- -- -- -- -- --     ◃ext′ p (function fn ts) = cong (function fn) (◃ext p ts)

-- -- -- -- -- --   instance SubstitutionExtensionalityVecTerm : ∀ {N} → SubstitutionExtensionality (flip Vec N ∘ Term)
-- -- -- -- -- --   SubstitutionExtensionality.◃ext (SubstitutionExtensionalityVecTerm {N}) = λ x → ◃ext′ x where
-- -- -- -- -- --     ◃ext′ : ∀ {m n} {f g : Fin m → Term n} → f ≐ g → ∀ {N} (t : Vec (Term m) N) → f ◃ t ≡ g ◃ t
-- -- -- -- -- --     ◃ext′ p [] = refl
-- -- -- -- -- --     ◃ext′ p (t ∷ ts) = cong₂ _∷_ (◃ext p t) (◃ext p ts)

-- -- -- -- -- -- _◇_ : ∀ {l m n : ℕ } → (f : Fin m → Term n) (g : Fin l → Term m) → Fin l → Term n
-- -- -- -- -- -- f ◇ g = (f ◃_) ∘ g

-- -- -- -- -- -- ≐-cong : ∀ {m n o} {f : m ⊸ n} {g} (h : _ ⊸ o) → f ≐ g → (h ◇ f) ≐ (h ◇ g)
-- -- -- -- -- -- ≐-cong h f≐g t = cong (h ◃_) (f≐g t)

-- -- -- -- -- -- ≐-sym : ∀ {m n} {f : m ⊸ n} {g} → f ≐ g → g ≐ f
-- -- -- -- -- -- ≐-sym f≐g = sym ∘ f≐g

-- -- -- -- -- -- module Sub where
-- -- -- -- -- --   record Fact1 (T : ℕ → Set) ⦃ _ : Substitution T ⦄ : Set where
-- -- -- -- -- --     field
-- -- -- -- -- --       fact1 : ∀ {n} → (t : T n) → i ◃ t ≡ t

-- -- -- -- -- --   open Fact1 ⦃ … ⦄ public

-- -- -- -- -- --   mutual

-- -- -- -- -- --     instance Fact1Term : Fact1 Term
-- -- -- -- -- --     Fact1.fact1 Fact1Term (i x) = refl
-- -- -- -- -- --     Fact1.fact1 Fact1Term leaf = refl
-- -- -- -- -- --     Fact1.fact1 Fact1Term (s fork t) = cong₂ _fork_ (fact1 s) (fact1 t)
-- -- -- -- -- --     Fact1.fact1 Fact1Term (function fn ts) = cong (function fn) (fact1 ts)

-- -- -- -- -- --     instance Fact1TermVec : ∀ {N} → Fact1 (flip Vec N ∘ Term)
-- -- -- -- -- --     Fact1.fact1 Fact1TermVec [] = refl
-- -- -- -- -- --     Fact1.fact1 Fact1TermVec (t ∷ ts) = cong₂ _∷_ (fact1 t) (fact1 ts)

-- -- -- -- -- --   record Fact2 (T : ℕ → Set) ⦃ _ : Substitution T ⦄ : Set where
-- -- -- -- -- --     field
-- -- -- -- -- --       -- ⦃ s ⦄ : Substitution T
-- -- -- -- -- --       fact2 : ∀ {l m n} → {f : Fin m → Term n} {g : _} (t : T l) → (f ◇ g) ◃ t ≡ f ◃ (g ◃ t)

-- -- -- -- -- --   open Fact2 ⦃ … ⦄ public

-- -- -- -- -- --   mutual

-- -- -- -- -- --     instance Fact2Term : Fact2 Term
-- -- -- -- -- --     -- Fact2.s Fact2Term = SubstitutionTerm
-- -- -- -- -- --     Fact2.fact2 Fact2Term (i x) = refl
-- -- -- -- -- --     Fact2.fact2 Fact2Term leaf = refl
-- -- -- -- -- --     Fact2.fact2 Fact2Term (s fork t) = cong₂ _fork_ (fact2 s) (fact2 t)
-- -- -- -- -- --     Fact2.fact2 Fact2Term {f = f} {g = g} (function fn ts) = cong (function fn) (fact2 {f = f} {g = g} ts) -- fact2 ts

-- -- -- -- -- --     instance Fact2TermVec : ∀ {N} → Fact2 (flip Vec N ∘ Term)
-- -- -- -- -- --     -- Fact2.s Fact2TermVec = SubstitutionVecTerm
-- -- -- -- -- --     Fact2.fact2 Fact2TermVec [] = refl
-- -- -- -- -- --     Fact2.fact2 Fact2TermVec (t ∷ ts) = cong₂ _∷_ (fact2 t) (fact2 ts)

-- -- -- -- -- --   fact3 : ∀ {l m n} (f : Fin m → Term n) (r : Fin l → Fin m) → (f ◇ (▸ r)) ≡ (f ∘ r)
-- -- -- -- -- --   fact3 f r = refl

-- -- -- -- -- -- ◃ext' : ∀ {m n o} {f : Fin m → Term n}{g : Fin m → Term o}{h} → f ≐ (h ◇ g) → ∀ (t : Term _) → f ◃ t ≡ h ◃ (g ◃ t)
-- -- -- -- -- -- ◃ext' p t = trans (◃ext p t) (Sub.fact2 t)

-- -- -- -- -- -- open import Data.Maybe using (Maybe; nothing; just; functor; maybe′; maybe)
-- -- -- -- -- -- open import Category.Monad
-- -- -- -- -- -- import Level
-- -- -- -- -- -- --open RawMonad (Data.Maybe.monad {Level.zero})
-- -- -- -- -- -- open import Data.Nat using (ℕ)

-- -- -- -- -- -- _<*>_ = _⊛_

-- -- -- -- -- -- mutual

-- -- -- -- -- --   instance CheckTerm : Check Term
-- -- -- -- -- --   Check.check CheckTerm x (i y) = i <$> thick? x y
-- -- -- -- -- --   Check.check CheckTerm x leaf = just leaf
-- -- -- -- -- --   Check.check CheckTerm x (s fork t) = _fork_ <$> check x s ⊛ check x t
-- -- -- -- -- --   Check.check CheckTerm x (function fn ts) = ⦇ (function fn) (check x ts) ⦈

-- -- -- -- -- --   instance CheckTermVec : ∀ {N} → Check (flip Vec N ∘ Term)
-- -- -- -- -- --   Check.check CheckTermVec x [] = just []
-- -- -- -- -- --   Check.check CheckTermVec x (t ∷ ts) = ⦇ check x t ∷ check x ts ⦈

-- -- -- -- -- -- _for_ : ∀ {n} (t' : Term n) (x : Fin (suc n)) → Fin (suc n) → Term n
-- -- -- -- -- -- (t' for x) y = maybe′ i t' (thick? x y)

-- -- -- -- -- -- open import Data.Product using () renaming (Σ to Σ₁)
-- -- -- -- -- -- open Σ₁ renaming (proj₁ to π₁; proj₂ to π₂)

-- -- -- -- -- -- Property⋆ : (m : ℕ) → Set1
-- -- -- -- -- -- Property⋆ m = ∀ {n} → (Fin m → Term n) → Set

-- -- -- -- -- -- Extensional : {m : ℕ} → Property⋆ m → Set
-- -- -- -- -- -- Extensional P = ∀ {m f g} → f ≐ g → P {m} f → P g

-- -- -- -- -- -- Property : (m : ℕ) → Set1
-- -- -- -- -- -- Property m = Σ₁ (Property⋆ m) Extensional

-- -- -- -- -- -- prop-id : ∀ {m n} {f : _ ⊸ n} {P : Property m} → π₁ P f → π₁ P (i ◇ f)
-- -- -- -- -- -- prop-id {_} {_} {f} {P'} Pf = π₂ P' (λ x → sym (Sub.fact1 (f x))) Pf

-- -- -- -- -- -- Unifies⋆ : ∀ {m} (s t : Term m) → Property⋆ m
-- -- -- -- -- -- Unifies⋆ s t f = f ◃ s ≡ f ◃ t

-- -- -- -- -- -- Unifies⋆V : ∀ {m N} (ss ts : Vec (Term m) N) → Property⋆ m
-- -- -- -- -- -- Unifies⋆V ss ts f = f ◃ ss ≡ f ◃ ts

-- -- -- -- -- -- open import Relation.Binary.PropositionalEquality renaming ([_] to [[_]])
-- -- -- -- -- -- open ≡-Reasoning

-- -- -- -- -- -- Unifies : ∀ {m} (s t : Term m) → Property m
-- -- -- -- -- -- Unifies s t = (λ {_} → Unifies⋆ s t) , λ {_} {f} {g} f≐g f◃s=f◃t →
-- -- -- -- -- --   begin
-- -- -- -- -- --     g ◃ s
-- -- -- -- -- --   ≡⟨ sym (◃ext f≐g s) ⟩
-- -- -- -- -- --     f ◃ s
-- -- -- -- -- --   ≡⟨ f◃s=f◃t ⟩
-- -- -- -- -- --     f ◃ t
-- -- -- -- -- --   ≡⟨ ◃ext f≐g t ⟩
-- -- -- -- -- --     g ◃ t
-- -- -- -- -- --   ∎

-- -- -- -- -- -- UnifiesV : ∀ {m} {N} (s t : Vec (Term m) N) → Property m
-- -- -- -- -- -- UnifiesV s t = (λ {_} → Unifies⋆V s t) , λ {_} {f} {g} f≐g f◃s=f◃t →
-- -- -- -- -- --   begin
-- -- -- -- -- --     g ◃ s
-- -- -- -- -- --   ≡⟨ sym (◃ext f≐g s) ⟩
-- -- -- -- -- --     f ◃ s
-- -- -- -- -- --   ≡⟨ f◃s=f◃t ⟩
-- -- -- -- -- --     f ◃ t
-- -- -- -- -- --   ≡⟨ ◃ext f≐g t ⟩
-- -- -- -- -- --     g ◃ t
-- -- -- -- -- --   ∎


-- -- -- -- -- -- _∧⋆_ : ∀{m} → (P Q : Property⋆ m) → Property⋆ m
-- -- -- -- -- -- P ∧⋆ Q = (λ f → P f × Q f)

-- -- -- -- -- -- -- open import Data.Product renaming (map to _***_)
-- -- -- -- -- -- open import Data.Product using (Σ)
-- -- -- -- -- -- open Σ

-- -- -- -- -- -- _∧_ : ∀{m} → (P Q : Property m) → Property m
-- -- -- -- -- -- P ∧ Q = (λ {_} f → π₁ P f × π₁ Q f) , λ {_} {_} {_} f≐g Pf×Qf → π₂ P f≐g (proj₁ Pf×Qf) , π₂ Q f≐g (proj₂ Pf×Qf)


-- -- -- -- -- -- _⇔⋆_ : ∀{m} → (P Q : Property⋆ m) → Set
-- -- -- -- -- -- P ⇔⋆ Q = ∀ {n} f → (P {n} f → Q f) × (Q f → P f)

-- -- -- -- -- -- _⇔_ : ∀{m} → (P Q : Property m) → Set
-- -- -- -- -- -- P ⇔ Q = ∀ {n} f → (π₁ P {n} f → π₁ Q f) × (π₁ Q f → π₁ P f)

-- -- -- -- -- -- switch⋆ : ∀ {m} (P Q : Property⋆ m) → P ⇔⋆ Q → Q ⇔⋆ P
-- -- -- -- -- -- switch⋆ _ _ P⇔Q f = proj₂ (P⇔Q f) , proj₁ (P⇔Q f)

-- -- -- -- -- -- switch : ∀ {m} (P Q : Property m) → P ⇔ Q → Q ⇔ P
-- -- -- -- -- -- switch _ _ P⇔Q f = proj₂ (P⇔Q f) , proj₁ (P⇔Q f)

-- -- -- -- -- -- open import Data.Empty

-- -- -- -- -- -- Nothing⋆ : ∀{m} → (P : Property⋆ m) → Set
-- -- -- -- -- -- Nothing⋆ P = ∀{n} f → P {n} f → ⊥

-- -- -- -- -- -- Nothing : ∀{m} → (P : Property m) → Set
-- -- -- -- -- -- Nothing P = ∀{n} f → π₁ P {n} f → ⊥

-- -- -- -- -- -- _[-◇⋆_] : ∀{m n} (P : Property⋆ m) (f : Fin m → Term n) → Property⋆ n
-- -- -- -- -- -- (P [-◇⋆ f ]) g = P (g ◇ f)

-- -- -- -- -- -- _[-◇_] : ∀{m n} (P : Property m) (f : Fin m → Term n) → Property n
-- -- -- -- -- -- P [-◇ f ] = (λ {_} g → π₁ P (g ◇ f)) , λ {_} {f'} {g'} f'≐g' Pf'◇f → π₂ P (◃ext f'≐g' ∘ f)  Pf'◇f

-- -- -- -- -- -- open import Function using (_∘_; id; case_of_; _$_; flip)
-- -- -- -- -- -- open import Data.Product using (curry; uncurry)

-- -- -- -- -- -- module Properties where
-- -- -- -- -- --   fact1 : ∀ {m} {s t : Term m} → (Unifies s t) ⇔ (Unifies t s)
-- -- -- -- -- --   fact1 _ = sym , sym


-- -- -- -- -- --   fact1'⋆ : ∀ {m} {s1 s2 t1 t2 : Term m}
-- -- -- -- -- --          → Unifies⋆ (s1 fork s2) (t1 fork t2) ⇔⋆ (Unifies⋆ s1 t1 ∧⋆ Unifies⋆ s2 t2)
-- -- -- -- -- --   fact1'⋆ f = deconstr _ _ _ _ , uncurry (cong₂ _fork_)
-- -- -- -- -- --     where deconstr : ∀ {m} (s1 s2 t1 t2 : Term m)
-- -- -- -- -- --                    → (s1 fork s2) ≡ (t1 fork t2)
-- -- -- -- -- --                    → (s1 ≡ t1) × (s2 ≡ t2)
-- -- -- -- -- --           deconstr s1 s2 .s1 .s2 refl = refl , refl

-- -- -- -- -- --   fact1' : ∀ {m} {s1 s2 t1 t2 : Term m}
-- -- -- -- -- --          → Unifies (s1 fork s2) (t1 fork t2) ⇔ (Unifies s1 t1 ∧ Unifies s2 t2)
-- -- -- -- -- --   fact1' f = deconstr _ _ _ _ , uncurry (cong₂ _fork_)
-- -- -- -- -- --     where deconstr : ∀ {m} (s1 s2 t1 t2 : Term m)
-- -- -- -- -- --                    → (s1 fork s2) ≡ (t1 fork t2)
-- -- -- -- -- --                    → (s1 ≡ t1) × (s2 ≡ t2)
-- -- -- -- -- --           deconstr s1 s2 .s1 .s2 refl = refl , refl

-- -- -- -- -- --   fact1'V : ∀ {m} {t₁ t₂ : Term m} {N} {ts₁ ts₂ : Vec (Term m) N}
-- -- -- -- -- --          → UnifiesV (t₁ ∷ ts₁) (t₂ ∷ ts₂) ⇔ (Unifies t₁ t₂ ∧ UnifiesV ts₁ ts₂)
-- -- -- -- -- --   fact1'V f = deconstr _ _ _ _ , uncurry (cong₂ _∷_)
-- -- -- -- -- --     where deconstr : ∀ {m} (t₁ t₂ : Term m) {N} (ts₁ ts₂ : Vec (Term m) N)
-- -- -- -- -- --                    → (t₁ Vec.∷ ts₁) ≡ (t₂ ∷ ts₂)
-- -- -- -- -- --                    → (t₁ ≡ t₂) × (ts₁ ≡ ts₂)
-- -- -- -- -- --           deconstr s1 _ s2! _ refl = refl , refl -- refl , refl


-- -- -- -- -- --   fact2⋆ : ∀ {m} (P Q : Property⋆ m) → P ⇔⋆ Q → Nothing⋆ P → Nothing⋆ Q
-- -- -- -- -- --   fact2⋆ P Q iff notp f q with iff f
-- -- -- -- -- --   ...                        | (p2q , q2p) = notp f (q2p q)

-- -- -- -- -- --   fact2 : ∀ {m} (P Q : Property m) → P ⇔ Q → Nothing P → Nothing Q
-- -- -- -- -- --   fact2 P Q iff notp f q with iff f
-- -- -- -- -- --   ...                       | (p2q , q2p) = notp f (q2p q)


-- -- -- -- -- --   fact3 : ∀ {m} {P : Property m} → P ⇔ (P [-◇ i ])
-- -- -- -- -- --   fact3 f = id , id

-- -- -- -- -- --   fact4 : ∀{m n} {P : Property m} (f : _ → Term n)
-- -- -- -- -- --           → Nothing P → Nothing (P [-◇ f ])
-- -- -- -- -- --   fact4 f nop g = nop (g ◇ f)

-- -- -- -- -- --   fact5⋆ : ∀{m n} (P Q : Property⋆ _) (f : m ⊸ n) → P ⇔⋆ Q → (P [-◇⋆ f ]) ⇔⋆ (Q [-◇⋆ f ])
-- -- -- -- -- --   fact5⋆ _ _ f P⇔Q f' = P⇔Q (f' ◇ f)

-- -- -- -- -- --   fact5 : ∀{m n} (P Q : Property _) (f : m ⊸ n) → P ⇔ Q → (P [-◇ f ]) ⇔ (Q [-◇ f ])
-- -- -- -- -- --   fact5 _ _ f P⇔Q f' = P⇔Q (f' ◇ f)

-- -- -- -- -- --   fact6 : ∀{m n} P {f g : m ⊸ n} → f ≐ g → (P [-◇ f ]) ⇔ (P [-◇ g ])
-- -- -- -- -- --   fact6 P f≐g h = π₂ P (≐-cong h f≐g) , π₂ P (≐-sym (≐-cong h f≐g))

-- -- -- -- -- -- _≤_ : ∀ {m n n'} (f : Fin m → Term n) (g : Fin m → Term n') → Set
-- -- -- -- -- -- f ≤ g = ∃ λ f' → f ≐ (f' ◇ g)

-- -- -- -- -- -- module Order where

-- -- -- -- -- --   reflex : ∀ {m n} {f : Fin m → Term n} → f ≤ f
-- -- -- -- -- --   reflex = i  , λ _ → sym (Sub.fact1 _)

-- -- -- -- -- --   transitivity : ∀ {l m n o} {f : Fin l → Term m}{g : _ → Term n}
-- -- -- -- -- --                              {h : _ → Term o}
-- -- -- -- -- --                    → f ≤ g → g ≤ h → f ≤ h
-- -- -- -- -- --   transitivity {l} {_} {_} {_} {f} {g} {h} (fg , pfg) (gh , pgh) =
-- -- -- -- -- --                    fg ◇ gh , proof
-- -- -- -- -- --     where
-- -- -- -- -- --       proof : (x : Fin l) → f x ≡ (λ x' → fg ◃ (gh x')) ◃ (h x)
-- -- -- -- -- --       proof x = trans z (sym (Sub.fact2 (h x)))
-- -- -- -- -- --         where z = trans (pfg x) (cong (fg ◃_) (pgh x))

-- -- -- -- -- --   i-max : ∀ {m n} (f : Fin m → Term n) → f ≤ i
-- -- -- -- -- --   i-max f = f , λ _ → refl

-- -- -- -- -- --   dist : ∀{l m n o}{f : Fin l → Term m}{g : _ → Term n}(h : Fin o → _) → f ≤ g → (f ◇ h) ≤ (g ◇ h)
-- -- -- -- -- --   dist h (fg , pfg) = fg  , λ x → trans (◃ext pfg (h x)) (Sub.fact2 (h x))

-- -- -- -- -- -- Max⋆ : ∀ {m} (P : Property⋆ m) → Property⋆ m
-- -- -- -- -- -- Max⋆ P f = P f × (∀ {n} f' → P {n} f' → f' ≤ f)

-- -- -- -- -- -- Max : ∀ {m} (P : Property m) → Property m
-- -- -- -- -- -- Max P' = (λ {_} → Max⋆ P) , λ {_} {_} {_} → lemma1
-- -- -- -- -- --   where
-- -- -- -- -- --     open Σ₁ P' renaming (proj₁ to P; proj₂ to Peq)
-- -- -- -- -- --     lemma1 : {m : ℕ} {f : Fin _ → Term m} {g : Fin _ → Term m} →
-- -- -- -- -- --              f ≐ g →
-- -- -- -- -- --              P f × ({n : ℕ} (f' : Fin _ → Term n) → P f' → f' ≤ f) →
-- -- -- -- -- --              P g × ({n : ℕ} (f' : Fin _ → Term n) → P f' → f' ≤ g)
-- -- -- -- -- --     lemma1 {_} {f} {g} f≐g (Pf , MaxPf) = Peq f≐g Pf , λ {_} → lemma2
-- -- -- -- -- --       where
-- -- -- -- -- --         lemma2 : ∀ {n} f' → P {n} f' → ∃ λ f0 → f' ≐ (f0 ◇ g)
-- -- -- -- -- --         lemma2 f' Pf' = f0 , λ x → trans (f'≐f0◇f x) (cong (f0 ◃_) (f≐g x))
-- -- -- -- -- --               where
-- -- -- -- -- --                 f0 = proj₁ (MaxPf f' Pf')
-- -- -- -- -- --                 f'≐f0◇f = proj₂ (MaxPf f' Pf')


-- -- -- -- -- -- module Max where
-- -- -- -- -- --   fact : ∀{m}(P Q : Property m) → P ⇔ Q → Max P ⇔ Max Q
-- -- -- -- -- --   fact {m} P Q a f =
-- -- -- -- -- --    (λ maxp → pq (proj₁ maxp) , λ f' → proj₂ maxp f' ∘ qp)
-- -- -- -- -- --     , λ maxq → qp (proj₁ maxq) , λ f'  → proj₂ maxq f' ∘ pq
-- -- -- -- -- --     where
-- -- -- -- -- --       pq : {n : ℕ} {f0 : Fin m → Term n} → (π₁ P f0 → π₁ Q f0)
-- -- -- -- -- --       pq {_} {f} =  proj₁ (a f)
-- -- -- -- -- --       qp : {n : ℕ} {f0 : Fin m → Term n} → (π₁ Q f0 → π₁ P f0)
-- -- -- -- -- --       qp {_} {f} = proj₂ (a f)

-- -- -- -- -- -- DClosed : ∀{m} (P : Property m) → Set
-- -- -- -- -- -- DClosed P = ∀ {n} f {o} g → f ≤ g → π₁ P {o} g → π₁ P {n} f


-- -- -- -- -- -- module DClosed where

-- -- -- -- -- --   fact1 : ∀ {m} s t → DClosed {m} (Unifies s t)
-- -- -- -- -- --   fact1 s t f g (f≤g , p) gs=gt =
-- -- -- -- -- --          begin
-- -- -- -- -- --          f ◃ s
-- -- -- -- -- --          ≡⟨ ◃ext' p s ⟩
-- -- -- -- -- --          f≤g ◃ (g ◃ s)
-- -- -- -- -- --          ≡⟨ cong (f≤g ◃_) gs=gt ⟩
-- -- -- -- -- --          f≤g ◃ (g ◃ t)
-- -- -- -- -- --          ≡⟨ sym (◃ext' p t) ⟩
-- -- -- -- -- --          f ◃ t
-- -- -- -- -- --          ∎

-- -- -- -- -- -- optimist : ∀ {l m n o} (a : Fin _ → Term n) (p : Fin _ → Term o)
-- -- -- -- -- --                  (q : Fin _ → Term l) (P Q : Property m)
-- -- -- -- -- --            → DClosed P → π₁ (Max (P [-◇ a ])) p
-- -- -- -- -- --            → π₁ (Max (Q [-◇ (p ◇ a) ])) q
-- -- -- -- -- --            → π₁ (Max ((P ∧ Q) [-◇ a ])) (q ◇ p)
-- -- -- -- -- -- optimist a p q P' Q' DCP (Ppa , pMax) (Qqpa , qMax) =
-- -- -- -- -- --      (Peq (sym ∘ Sub.fact2 ∘ a) (DCP (q ◇ (p ◇ a)) (p ◇ a) (q , λ _ → refl) Ppa)
-- -- -- -- -- --       , Qeq (sym ∘ Sub.fact2 ∘ a) Qqpa )
-- -- -- -- -- --      , λ {_} → aux
-- -- -- -- -- --   where
-- -- -- -- -- --     open Σ₁ P' renaming (proj₁ to P; proj₂ to Peq)
-- -- -- -- -- --     open Σ₁ Q' renaming (proj₁ to Q; proj₂ to Qeq)
-- -- -- -- -- --     aux : ∀ {n} (f : _ → Term n) → P (f ◇ a) × Q (f ◇ a) → f ≤ (q ◇ p)
-- -- -- -- -- --     aux f (Pfa , Qfa) = h ,
-- -- -- -- -- --                         λ x → trans (f≐g◇p x) (◃ext' g≐h◇q (p x))
-- -- -- -- -- --       where
-- -- -- -- -- --         one = pMax f Pfa
-- -- -- -- -- --         g = proj₁ one
-- -- -- -- -- --         f≐g◇p = proj₂ one
-- -- -- -- -- --         Qgpa : Q (g ◇ (p ◇ a))
-- -- -- -- -- --         Qgpa = Qeq (λ x → ◃ext' f≐g◇p (a x)) Qfa
-- -- -- -- -- --         g≤q = qMax g Qgpa
-- -- -- -- -- --         h = proj₁ g≤q
-- -- -- -- -- --         g≐h◇q = proj₂ g≤q


-- -- -- -- -- -- module failure-propagation where

-- -- -- -- -- --   first⋆ : ∀ {m n} (a : _ ⊸ n) (P Q : Property⋆ m) →
-- -- -- -- -- --          Nothing⋆ (P [-◇⋆ a ]) → Nothing⋆ ((P ∧⋆ Q) [-◇⋆ a ])
-- -- -- -- -- --   first⋆ a P' Q' noP-a f (Pfa , Qfa) = noP-a f Pfa

-- -- -- -- -- --   first : ∀ {m n} (a : _ ⊸ n) (P Q : Property m) →
-- -- -- -- -- --          Nothing (P [-◇ a ]) → Nothing ((P ∧ Q) [-◇ a ])
-- -- -- -- -- --   first a P' Q' noP-a f (Pfa , Qfa) = noP-a f Pfa

-- -- -- -- -- --   second⋆ : ∀ {m n o} (a : _ ⊸ n) (p : _ ⊸ o)(P : Property⋆ m)(Q : Property m) →
-- -- -- -- -- --              (Max⋆ (P [-◇⋆ a ])) p → Nothing⋆ (π₁ Q [-◇⋆ (p ◇ a)])
-- -- -- -- -- --              → Nothing⋆ ((P ∧⋆ π₁ Q) [-◇⋆ a ])
-- -- -- -- -- --   second⋆ a p P' Q' (Ppa , pMax) noQ-p◇a f (Pfa , Qfa) = noQ-p◇a g Qgpa
-- -- -- -- -- --        where
-- -- -- -- -- --          f≤p = pMax f Pfa
-- -- -- -- -- --          g = proj₁ f≤p
-- -- -- -- -- --          f≐g◇p = proj₂ f≤p
-- -- -- -- -- --          Qgpa : π₁ Q' (g ◇ (p ◇ a))
-- -- -- -- -- --          Qgpa = π₂ Q' (◃ext' f≐g◇p ∘ a)  Qfa

-- -- -- -- -- --   second : ∀ {m n o} (a : _ ⊸ n) (p : _ ⊸ o)(P Q : Property m) →
-- -- -- -- -- --              π₁ (Max (P [-◇ a ])) p → Nothing (Q [-◇ (p ◇ a)])
-- -- -- -- -- --              → Nothing ((P ∧ Q) [-◇ a ])
-- -- -- -- -- --   second a p P' Q' (Ppa , pMax) noQ-p◇a f (Pfa , Qfa) = noQ-p◇a g Qgpa
-- -- -- -- -- --        where
-- -- -- -- -- --          f≤p = pMax f Pfa
-- -- -- -- -- --          g = proj₁ f≤p
-- -- -- -- -- --          f≐g◇p = proj₂ f≤p
-- -- -- -- -- --          Qgpa : π₁ Q' (g ◇ (p ◇ a))
-- -- -- -- -- --          Qgpa = π₂ Q' (◃ext' f≐g◇p ∘ a)  Qfa


-- -- -- -- -- -- trivial-problem : ∀ {m n t} {f : m ⊸ n} → (Max⋆ ((Unifies⋆ t t) [-◇⋆ f ])) i
-- -- -- -- -- -- trivial-problem = refl , λ f' _ → f' , λ _ → refl

-- -- -- -- -- -- trivial-problemV : ∀ {m n N} {t : Vec (Term _) N} {f : m ⊸ n} → (Max⋆ ((Unifies⋆V t t) [-◇⋆ f ])) i
-- -- -- -- -- -- trivial-problemV = refl , λ f' _ → f' , λ _ → refl

-- -- -- -- -- -- open import Data.Sum

-- -- -- -- -- -- var-elim : ∀ {m} (x : Fin (suc m)) (t' : Term _)
-- -- -- -- -- --               → π₁ (Max ((Unifies (i x) ((▸ (thin x) ◃_) t')))) (t' for x)
-- -- -- -- -- -- var-elim x t' = first , \{_} → second
-- -- -- -- -- --   where
-- -- -- -- -- --     lemma : ∀{m}(x : Fin (suc m)) t → i ≐ ((t for x) ◇ (▸ (thin x)))
-- -- -- -- -- --     lemma x t x' = sym (cong (maybe i t) (Thick.half2 x _ x' refl))
-- -- -- -- -- --     first = begin
-- -- -- -- -- --              (t' for x) ◃ (i x) ≡⟨ cong (maybe i t') (Thick.half1 x) ⟩
-- -- -- -- -- --              t'                 ≡⟨ sym (Sub.fact1 t') ⟩
-- -- -- -- -- --              i ◃ t'             ≡⟨ ◃ext' (lemma x t') t' ⟩
-- -- -- -- -- --              (t' for x) ◃ ((▸ (thin x) ◃_) t') ∎

-- -- -- -- -- --     second : ∀ {n} (f : _ ⊸ n) → f x ≡ f ◃ ((▸ (thin x) ◃_) t') → f ≤ (t' for x)
-- -- -- -- -- --     second f Unifiesf = (f ∘ thin x) , third
-- -- -- -- -- --         where
-- -- -- -- -- --           third : ((x' : Fin _) →  f x' ≡ (f ∘ thin x) ◃ (maybe′ i t' (thick? x x')))
-- -- -- -- -- --           third x' with thick? x x' | Thick.fact1 x x' (thick? x x') refl
-- -- -- -- -- --           third .x | .nothing | inj₁ (refl , refl)  =
-- -- -- -- -- --                                        sym (begin
-- -- -- -- -- --                                            (f ∘ thin x) ◃ t'  ≡⟨ cong (λ g → (g ◃_) t') (sym (Sub.fact3 f (thin x))) ⟩
-- -- -- -- -- --                                            (f ◇ (▸ (thin x))) ◃ t' ≡⟨ Sub.fact2 {-f (▸ (thin x))-} t' ⟩
-- -- -- -- -- --                                            f ◃ ((▸ (thin x) ◃_) t') ≡⟨ sym Unifiesf ⟩
-- -- -- -- -- --                                            f x ∎)
-- -- -- -- -- --           third x' | .(just y) | inj₂ (y , ( thinxy≡x' , refl))  = sym (cong f thinxy≡x')

-- -- -- -- -- -- var-elim-i : ∀ {m} (x : Fin (suc m)) (t' : Term _)
-- -- -- -- -- --               → π₁ (Max ((Unifies (i x) ((▸ (thin x) ◃_) t')))) (i ◇ (t' for x))
-- -- -- -- -- -- var-elim-i {m} x t = prop-id {_} {_} {t for x} {Max (Unifies (i x) ((▸ (thin x) ◃_) t))} (var-elim {m} x t)

-- -- -- -- -- -- var-elim-i-≡ : ∀ {m} {t'} (x : Fin (suc m)) t1  → t1 ≡ (i ∘ thin x) ◃ t' → π₁ (Max (Unifies (i x) t1)) (i ◇ (t' for x))
-- -- -- -- -- -- var-elim-i-≡ {_} {t'} x .((i ∘ thin x) ◃ t') refl = var-elim-i x t'

-- -- -- -- -- -- ◇-assoc : ∀ {l m n o} (f : l ⊸ m) (g : n ⊸ _) (h : o ⊸ _) →
-- -- -- -- -- --                (f ◇ (g ◇ h)) ≐ ((f ◇ g) ◇ h)
-- -- -- -- -- -- ◇-assoc f g h x = sym (Sub.fact2 (h x))

-- -- -- -- -- -- bind-assoc : ∀ {l m n o} (f : l ⊸ m) (g : n ⊸ _) (h : o ⊸ _) t → (f ◇ g) ◃ (h ◃ t) ≡ (f ◇ (g ◇ h)) ◃ t
-- -- -- -- -- -- bind-assoc f g h t = sym (begin
-- -- -- -- -- --            (f ◇ (g ◇ h)) ◃ t  ≡⟨ ◃ext (◇-assoc f g h) t ⟩
-- -- -- -- -- --            ((f ◇ g) ◇ h) ◃ t  ≡⟨ Sub.fact2 ⦃ SubstitutionTerm ⦄ ⦃ Sub.Fact2Term ⦄ {f = (f ◇ g)} {g = h} {-(f ◇ g) h-} t ⟩
-- -- -- -- -- --            (f ◇ g) ◃ (h  ◃ t)
-- -- -- -- -- --                               ∎)
