
Specification of Type Theory (from the HoTT book)

```agda
module TypeTheory-2 where
```

```agda
module FormalTypeTheory where
  open import Preliminary

  weakenFinFrom : âˆ€ {N} â†’ Fin (suc N) â†’ Fin N â†’ Fin (suc N)
  weakenFinFrom zero x = suc x
  weakenFinFrom (suc from) zero = zero
  weakenFinFrom (suc from) (suc x) = suc (weakenFinFrom from x)

  {- You are a pigeon. There are some pigeon holes labeled 0,1,...,N. You are given a particular pigeon hole, i. One of the holes that you are not given, labeled h, is removed, and the pigeon holes are relabeled 0,1,...,N-1. What is the new label on your pigeon hole?  -}
  instantiateFinAt : âˆ€ {N} {h i : Fin (suc N)} â†’ h â‰¢ i â†’ Fin N
  instantiateFinAt {zero} {zero} {zero} hâ‰¢i = âŠ¥-elim (hâ‰¢i refl)
  instantiateFinAt {zero} {zero} {suc ()} _
  instantiateFinAt {zero} {suc ()} {_} _
  instantiateFinAt {suc _} {_} {zero} _ = zero -- my label stays at 0
  instantiateFinAt {suc _} {zero} {suc i} _ = i -- my label shifts down
  instantiateFinAt {suc _} {suc h} {suc i} shâ‰¢si =
    let hâ‰¢i : h â‰¢ i -- the hole lower than mine is not the same as the hole lower than the one removed
        hâ‰¢i = Î» {refl â†’ shâ‰¢si refl}
    in
    suc (instantiateFinAt hâ‰¢i) -- my label is one more then the one lower than me after the change

  Universe = Nat

  data Complexity : Set where
    c : âˆ€ {N} â†’ Vec Complexity N â†’ Complexity

  data Term (N : Nat) : Set where
    ğ’° : Universe â†’ Term N
    ğ“‹ : Fin N â†’ Term N
    Î F : Term N â†’ Term (suc N) â†’ Term N
    Î I : Term (suc N) â†’ Term N
    Î E : Term N â†’ Term N â†’ Term N
    Î£F : Term N â†’ Term (suc N) â†’ Term N
    Î£I : Term N â†’ Term N â†’ Term N
    Î£E : Term (suc N) â†’ Term (suc (suc N)) â†’ Term N â†’ Term N
    +F : Term N â†’ Term N â†’ Term N
    +IL : Term N â†’ Term N
    +IR : Term N â†’ Term N
    +E : Term (suc N) â†’ Term (suc N) â†’ Term (suc N) â†’ Term N â†’ Term N
    ğŸ˜F : Term N
    ğŸ˜E : Term (suc N) â†’ Term N â†’ Term N
    ğŸ™F : Term N
    ğŸ™I : Term N
    ğŸ™E : Term (suc N) â†’ Term N â†’ Term N â†’ Term N
    â„•F : Term N
    â„•IZ : Term N
    â„•IS : Term N â†’ Term N
    â„•E : Term (suc N) â†’ Term N â†’ Term (suc (suc N)) â†’ Term N â†’ Term N
    =F : Term N â†’ Term N â†’ Term N â†’ Term N
    =I : Term N â†’ Term N
    =E : Term (suc (suc (suc N))) â†’ Term (suc N) â†’ Term N â†’ Term N â†’ Term N â†’ Term N

  weakenTermFrom : âˆ€ {N} â†’ Fin (suc N) â†’ Term N â†’ Term (suc N)
  weakenTermFrom from (ğ’° â„“) =
                       ğ’° â„“
  weakenTermFrom from (ğ“‹ v) =
                       ğ“‹ (weakenFinFrom from v)
  weakenTermFrom from (Î F tâ‚ tâ‚‚) =
                       Î F (weakenTermFrom from tâ‚)
                          (weakenTermFrom (suc from) tâ‚‚)
  weakenTermFrom from (Î I tâ‚) =
                       Î I (weakenTermFrom (suc from) tâ‚)
  weakenTermFrom from (Î E tâ‚ tâ‚‚) =
                       Î E (weakenTermFrom from tâ‚)
                          (weakenTermFrom from tâ‚‚)
  weakenTermFrom from (Î£F tâ‚ tâ‚‚) =
                       Î£F (weakenTermFrom from tâ‚)
                          (weakenTermFrom (suc from) tâ‚‚)
  weakenTermFrom from (Î£I tâ‚ tâ‚‚) =
                       Î£I (weakenTermFrom from tâ‚)
                          (weakenTermFrom from tâ‚‚)
  weakenTermFrom from (Î£E tâ‚ tâ‚‚ tâ‚ƒ) =
                       Î£E (weakenTermFrom (suc from) tâ‚)
                          (weakenTermFrom (suc (suc from)) tâ‚‚)
                          (weakenTermFrom from tâ‚ƒ)
  weakenTermFrom from (+F tâ‚ tâ‚‚) =
                       +F (weakenTermFrom from tâ‚)
                          (weakenTermFrom from tâ‚‚)
  weakenTermFrom from (+IL tâ‚) =
                       +IL (weakenTermFrom from tâ‚)
  weakenTermFrom from (+IR tâ‚) =
                       +IR (weakenTermFrom from tâ‚)
  weakenTermFrom from (+E tâ‚ tâ‚‚ tâ‚ƒ tâ‚„) =
                       +E (weakenTermFrom (suc from) tâ‚)
                          (weakenTermFrom (suc from) tâ‚‚)
                          (weakenTermFrom (suc from) tâ‚ƒ)
                          (weakenTermFrom from tâ‚„)
  weakenTermFrom from ğŸ˜F =
                      ğŸ˜F
  weakenTermFrom from (ğŸ˜E tâ‚ tâ‚‚) =
                       ğŸ˜E (weakenTermFrom (suc from) tâ‚)
                          (weakenTermFrom from tâ‚‚)
  weakenTermFrom from ğŸ™F =
                      ğŸ™F
  weakenTermFrom from ğŸ™I =
                      ğŸ™I
  weakenTermFrom from (ğŸ™E tâ‚ tâ‚‚ tâ‚ƒ) =
                       ğŸ™E (weakenTermFrom (suc from) tâ‚)
                          (weakenTermFrom from tâ‚‚)
                          (weakenTermFrom from tâ‚ƒ)
  weakenTermFrom from â„•F =
                      â„•F
  weakenTermFrom from â„•IZ =
                      â„•IZ
  weakenTermFrom from (â„•IS tâ‚) =
                       â„•IS (weakenTermFrom from tâ‚)
  weakenTermFrom from (â„•E tâ‚ tâ‚‚ tâ‚ƒ tâ‚„) =
                       â„•E (weakenTermFrom (suc from) tâ‚)
                          (weakenTermFrom from tâ‚‚)
                          (weakenTermFrom (suc (suc from)) tâ‚ƒ)
                          (weakenTermFrom from tâ‚„)
  weakenTermFrom from (=F tâ‚ tâ‚‚ tâ‚ƒ) =
                       =F (weakenTermFrom from tâ‚)
                          (weakenTermFrom from tâ‚‚)
                          (weakenTermFrom from tâ‚ƒ)
  weakenTermFrom from (=I tâ‚) =
                       =I (weakenTermFrom from tâ‚)
  weakenTermFrom from (=E tâ‚ tâ‚‚ tâ‚ƒ tâ‚„ tâ‚…) =
                       =E (weakenTermFrom (suc (suc (suc from))) tâ‚)
                          (weakenTermFrom (suc from) tâ‚‚)
                          (weakenTermFrom from tâ‚ƒ)
                          (weakenTermFrom from tâ‚„)
                          (weakenTermFrom from tâ‚…)

  instantiateTerm : âˆ€ {N} â†’ Fin (suc N) â†’ Term N â†’ Term (suc N) â†’ Term N
  instantiateTerm at Ï (ğ’° â„“) =
                        ğ’° â„“
  instantiateTerm at Ï (ğ“‹ v) with at == v
  â€¦ | yes _ = Ï
  â€¦ | no atâ‰ v = ğ“‹ (instantiateFinAt atâ‰ v)
  instantiateTerm at Ï (Î F tâ‚ tâ‚‚) =
                        Î F (instantiateTerm at Ï tâ‚)
                           (instantiateTerm (suc at) (weakenTermFrom zero Ï) tâ‚‚)
  instantiateTerm at Ï (Î I tâ‚) =
                        Î I (instantiateTerm (suc at) (weakenTermFrom zero Ï) tâ‚)
  instantiateTerm at Ï (Î E tâ‚ tâ‚‚) =
                        Î E (instantiateTerm at Ï tâ‚)
                           (instantiateTerm at Ï tâ‚‚)
  instantiateTerm at Ï (Î£F tâ‚ tâ‚‚) =
                        Î£F (instantiateTerm at Ï tâ‚)
                           (instantiateTerm (suc at) (weakenTermFrom zero Ï) tâ‚‚)
  instantiateTerm at Ï (Î£I tâ‚ tâ‚‚) =
                        Î£I (instantiateTerm at Ï tâ‚)
                           (instantiateTerm at Ï tâ‚‚)
  instantiateTerm at Ï (Î£E tâ‚ tâ‚‚ tâ‚ƒ) =
                        Î£E (instantiateTerm (suc at) (weakenTermFrom zero Ï) tâ‚)
                           (instantiateTerm (suc (suc at)) (weakenTermFrom zero (weakenTermFrom zero Ï)) tâ‚‚)
                           (instantiateTerm at Ï tâ‚ƒ)
  instantiateTerm at Ï (+F tâ‚ tâ‚‚) =
                        +F (instantiateTerm at Ï tâ‚)
                           (instantiateTerm at Ï tâ‚‚)
  instantiateTerm at Ï (+IL tâ‚) =
                        +IL (instantiateTerm at Ï tâ‚)
  instantiateTerm at Ï (+IR tâ‚) =
                        +IR (instantiateTerm at Ï tâ‚)
  instantiateTerm at Ï (+E tâ‚ tâ‚‚ tâ‚ƒ tâ‚„) =
                        +E (instantiateTerm (suc at) (weakenTermFrom zero Ï) tâ‚)
                           (instantiateTerm (suc at) (weakenTermFrom zero Ï) tâ‚‚)
                           (instantiateTerm (suc at) (weakenTermFrom zero Ï) tâ‚ƒ)
                           (instantiateTerm at Ï tâ‚„)
  instantiateTerm at Ï ğŸ˜F =
                       ğŸ˜F
  instantiateTerm at Ï (ğŸ˜E tâ‚ tâ‚‚) =
                        ğŸ˜E (instantiateTerm (suc at) (weakenTermFrom zero Ï) tâ‚)
                           (instantiateTerm at Ï tâ‚‚)
  instantiateTerm at Ï ğŸ™F =
                       ğŸ™F
  instantiateTerm at Ï ğŸ™I =
                       ğŸ™I
  instantiateTerm at Ï (ğŸ™E tâ‚ tâ‚‚ tâ‚ƒ) =
                        ğŸ™E (instantiateTerm (suc at) (weakenTermFrom zero Ï) tâ‚)
                           (instantiateTerm at Ï tâ‚‚)
                           (instantiateTerm at Ï tâ‚ƒ)
  instantiateTerm at Ï â„•F =
                       â„•F
  instantiateTerm at Ï â„•IZ =
                       â„•IZ
  instantiateTerm at Ï (â„•IS tâ‚) =
                        â„•IS (instantiateTerm at Ï tâ‚)
  instantiateTerm at Ï (â„•E tâ‚ tâ‚‚ tâ‚ƒ tâ‚„) =
                        â„•E (instantiateTerm (suc at) (weakenTermFrom zero Ï) tâ‚)
                           (instantiateTerm at Ï tâ‚‚)
                           (instantiateTerm (suc (suc at)) (weakenTermFrom zero (weakenTermFrom zero Ï)) tâ‚ƒ)
                           (instantiateTerm at Ï tâ‚„)
  instantiateTerm at Ï (=F tâ‚ tâ‚‚ tâ‚ƒ) =
                        =F (instantiateTerm at Ï tâ‚)
                           (instantiateTerm at Ï tâ‚‚)
                           (instantiateTerm at Ï tâ‚ƒ)
  instantiateTerm at Ï (=I tâ‚) =
                        =I (instantiateTerm at Ï tâ‚)
  instantiateTerm at Ï (=E tâ‚ tâ‚‚ tâ‚ƒ tâ‚„ tâ‚…) =
                        =E (instantiateTerm (suc (suc (suc at))) (weakenTermFrom zero (weakenTermFrom zero (weakenTermFrom zero Ï))) tâ‚)
                           (instantiateTerm (suc at) (weakenTermFrom zero Ï) tâ‚‚)
                           (instantiateTerm at Ï tâ‚ƒ)
                           (instantiateTerm at Ï tâ‚„)
                           (instantiateTerm at Ï tâ‚…)

  data _ctxâ‹–_ : Nat â†’ Complexity â†’ Set

  -- Î“ âŠ¢ a : A â‹– Ï‡ = a proves A given Î“, with complexity Ï‡
  data _âŠ¢_âˆ¶_â‹–_ {N Ï‡} (Î“ : N ctxâ‹– Ï‡) : Term N â†’ Term N â†’ Complexity â†’ Set

  -- Î“ âŠ¢ a : A = a is a proof of A given Î“
  _âŠ¢_âˆ¶_ : âˆ€ {N Ï‡} (Î“ : N ctxâ‹– Ï‡) â†’ Term N â†’ Term N â†’ Set
  Î“ âŠ¢ a âˆ¶ A = âˆƒ (Î“ âŠ¢ a âˆ¶ A â‹–_)

  -- Î“ âŠ¨ A = there is a proof of A
  _âŠ¨_ : âˆ€ {N Ï‡} (Î“ : N ctxâ‹– Ï‡) â†’ Term N â†’ Set
  Î“ âŠ¨ A = âˆƒ (Î“ âŠ¢_âˆ¶ A)

  Ï‡-measure : Complexity â†’ Nat
  Î´-measure : âˆ€ {N} â†’ Vec Complexity N â†’ Nat

  Ï‡-measure (c {N} Î´) = Î´-measure Î´

  Î´-measure {.0} [] = zero
  Î´-measure {.(suc _)} (Ï‡ âˆ· Î´) = suc (Ï‡-measure Ï‡ + Î´-measure Î´)

  _âŠ¨_â‰¼_ : âˆ€ {N Ï‡} (Î“ : N ctxâ‹– Ï‡) â†’ Term N â†’ Nat â†’ Set
  Î“ âŠ¨ A â‰¼ Î´ = âˆƒ Î» a â†’ âˆƒ Î» Ï‡ â†’ Ï‡-measure Ï‡ â‰¤ Î´ Ã— Î“ âŠ¢ a âˆ¶ A â‹– Ï‡

  infixl 25 _,,_

  data _ctxâ‹–_ where
    [] : zero ctxâ‹– c []
    _,,_ : âˆ€ {N â„“ A Î´Î“ Î´A} â†’
                (Î“ : N ctxâ‹– Î´Î“) â†’ Î“ âŠ¢ A âˆ¶ ğ’° â„“ â‹– Î´A â†’
              suc N ctxâ‹– c (Î´Î“ âˆ· Î´A âˆ· [])

  _at_ : âˆ€ {N Ï‡} â†’ N ctxâ‹– Ï‡ â†’ Fin N â†’ Term N
  _,,_ {A = A} Î“ Î³ at zero = weakenTermFrom zero A
  (Î“ ,, _) at suc n = weakenTermFrom zero (Î“ at n)

  data _âŠ¢_âˆ¶_â‹–_ {N Ï‡} (Î“ : N ctxâ‹– Ï‡) where
    ğ’°I : âˆ€ â„“ â†’
      Î“ âŠ¢ ğ’° â„“ âˆ¶ ğ’° (suc â„“) â‹– c []
    ğ’°C : âˆ€ {â„“ A Î´A} â†’
      Î“ âŠ¢ A âˆ¶ ğ’° â„“ â‹– Î´A â†’
      Î“ âŠ¢ A âˆ¶ ğ’° (suc â„“) â‹– c (Î´A âˆ· [])
    Î F : âˆ€ {â„“ A B Î´A Î´B} â†’
        (âŠ¢A : Î“ âŠ¢ A âˆ¶ ğ’° â„“ â‹– Î´A) â†’
        Î“ ,, âŠ¢A âŠ¢ B âˆ¶ ğ’° â„“ â‹– Î´B â†’
      Î“ âŠ¢ Î F A B âˆ¶ ğ’° â„“ â‹– c (Î´A âˆ· Î´B âˆ· [])
    Î I : âˆ€ {â„“ A b B Î´A Î´b} â†’
      (âŠ¢A : Î“ âŠ¢ A âˆ¶ ğ’° â„“ â‹– Î´A) â†’
      Î“ ,, âŠ¢A âŠ¢ b âˆ¶ B â‹– Î´b â†’
      Î“ âŠ¢ Î I b âˆ¶ Î F A B â‹– c (Î´b âˆ· [])
    Î E : âˆ€ {f Î´f A a Î´a B Ba} â†’
      Î“ âŠ¢ f âˆ¶ Î F A B â‹– Î´f â†’ Î“ âŠ¢ a âˆ¶ A â‹– Î´a â†’
      instantiateTerm zero a B â‰¡ Ba â†’
      Î“ âŠ¢ Î E f a âˆ¶ Ba â‹– c (Î´f âˆ· Î´a âˆ· [])
    Î£F : âˆ€ {â„“ A Î´A B Î´B} â†’
      (âŠ¢A : Î“ âŠ¢ A âˆ¶ ğ’° â„“ â‹– Î´A) â†’ Î“ ,, âŠ¢A âŠ¢ B âˆ¶ ğ’° â„“ â‹– Î´B â†’
      Î“ âŠ¢ Î£F A B âˆ¶ ğ’° â„“ â‹– c (Î´A âˆ· Î´B âˆ· [])
    Î£I : âˆ€ {â„“ A Î´A a Î´a B Î´B b Î´b} â†’
      (âŠ¢A : Î“ âŠ¢ A âˆ¶ ğ’° â„“ â‹– Î´A) â†’
      Î“ ,, âŠ¢A âŠ¢ B âˆ¶ ğ’° â„“ â‹– Î´B â†’ Î“ âŠ¢ a âˆ¶ A â‹– Î´a â†’ Î“ âŠ¢ b âˆ¶ instantiateTerm zero a B â‹– Î´b â†’
      Î“ âŠ¢ Î£I a b âˆ¶ Î£F A B â‹– c (Î´a âˆ· Î´b âˆ· [])
    Î£E : âˆ€ {â„“ Î´z A Î´A B Î´B C Î´C g Î´g p Î´p Cp} â†’
        (z : Î“ âŠ¢ Î£F A B âˆ¶ ğ’° â„“ â‹– Î´z) â†’
        Î“ ,, z âŠ¢ C âˆ¶ ğ’° â„“ â‹– Î´C â†’
        (âŠ¢A : Î“ âŠ¢ A âˆ¶ ğ’° â„“ â‹– Î´A) â†’
        (âŠ¢B : Î“ ,, âŠ¢A âŠ¢ B âˆ¶ ğ’° â„“ â‹– Î´B) â†’
        Î“ ,, âŠ¢A ,, âŠ¢B âŠ¢ g âˆ¶ instantiateTerm (suc (suc zero))
                                            (Î£I (ğ“‹ (suc zero)) (ğ“‹ zero))
                                            (weakenTermFrom zero (weakenTermFrom zero C)) â‹– Î´g â†’
        Î“ âŠ¢ p âˆ¶ Î£F A B â‹– Î´p â†’
        Cp â‰¡ instantiateTerm zero p C â†’
      Î“ âŠ¢ Î£E C g p âˆ¶ Cp â‹– c (Î´C âˆ· Î´g âˆ· Î´p âˆ· [])
    +F : âˆ€ {â„“ A Î´A B Î´B} â†’
      Î“ âŠ¢ A âˆ¶ ğ’° â„“ â‹– Î´A â†’ Î“ âŠ¢ B âˆ¶ ğ’° â„“ â‹– Î´B â†’
      Î“ âŠ¢ +F A B âˆ¶ ğ’° â„“ â‹– c (Î´A âˆ· Î´B âˆ· [])
    +IL : âˆ€ {â„“ A Î´A a Î´a B Î´B} â†’
      Î“ âŠ¢ A âˆ¶ ğ’° â„“ â‹– Î´A â†’ Î“ âŠ¢ B âˆ¶ ğ’° â„“ â‹– Î´B â†’ Î“ âŠ¢ a âˆ¶ A â‹– Î´a â†’
      Î“ âŠ¢ +IL a âˆ¶ +F A B â‹– Î´a
    +IR : âˆ€ {â„“ A Î´A b Î´b B Î´B} â†’
      Î“ âŠ¢ A âˆ¶ ğ’° â„“ â‹– Î´A â†’ Î“ âŠ¢ B âˆ¶ ğ’° â„“ â‹– Î´B â†’ Î“ âŠ¢ b âˆ¶ B â‹– Î´b â†’
      Î“ âŠ¢ +IR b âˆ¶ +F A B â‹– Î´b
    +E : âˆ€ {â„“ Î´z A Î´A B Î´B C Î´C c' Î´c d Î´d e Î´e Ce} â†’
        (âŠ¢z : Î“ âŠ¢ +F A B âˆ¶ ğ’° â„“ â‹– Î´z) â†’
        (âŠ¢A : Î“ âŠ¢ A âˆ¶ ğ’° â„“ â‹– Î´A) â†’
        (âŠ¢B : Î“ âŠ¢ B âˆ¶ ğ’° â„“ â‹– Î´B) â†’
        Î“ ,, âŠ¢z âŠ¢ C âˆ¶ ğ’° â„“ â‹– Î´C â†’
        Î“ ,, âŠ¢A âŠ¢ c' âˆ¶ instantiateTerm (suc zero)
                                      (+IL (ğ“‹ zero))
                                      (weakenTermFrom zero C) â‹– Î´c â†’
        Î“ ,, âŠ¢B âŠ¢ d âˆ¶ instantiateTerm (suc zero)
                                      (+IR (ğ“‹ zero))
                                      (weakenTermFrom zero C) â‹– Î´d â†’
        Î“ âŠ¢ e âˆ¶ +F A B â‹– Î´e â†’
        instantiateTerm zero e C â‰¡ Ce â†’
      Î“ âŠ¢ +E C c' d e âˆ¶ Ce â‹– c (Î´C âˆ· Î´c âˆ· Î´d âˆ· Î´e âˆ· [])
    ğŸ˜F : âˆ€ {â„“} â†’
      Î“ âŠ¢ ğŸ˜F âˆ¶ ğ’° â„“ â‹– c []
    ğŸ˜E : âˆ€ {â„“ Î´z C Î´C a Î´a Ca} â†’
      (z : Î“ âŠ¢ ğŸ˜F âˆ¶ ğ’° â„“ â‹– Î´z) â†’
      Î“ ,, z âŠ¢ C âˆ¶ ğ’° â„“ â‹– Î´C â†’ Î“ âŠ¢ a âˆ¶ ğŸ˜F â‹– Î´a â†’
      instantiateTerm zero a C â‰¡ Ca â†’
      Î“ âŠ¢ ğŸ˜E C a âˆ¶ Ca â‹– c (Î´C âˆ· Î´a âˆ· [])
    ğŸ™F : âˆ€ {â„“} â†’
      Î“ âŠ¢ ğŸ™F âˆ¶ ğ’° â„“ â‹– c []
    ğŸ™I :
      Î“ âŠ¢ ğŸ™I âˆ¶ ğŸ™F â‹– c []
    ğŸ™E : âˆ€ {â„“ C Î´C c' Î´c' a Î´a Ca} â†’
      Î“ ,, (ğŸ™F {â„“ = â„“}) âŠ¢ C âˆ¶ ğ’° â„“ â‹– Î´C â†’ Î“ âŠ¢ c' âˆ¶ instantiateTerm zero ğŸ™I C â‹– Î´c' â†’ Î“ âŠ¢ a âˆ¶ ğŸ™F â‹– Î´a â†’
      instantiateTerm zero a C â‰¡ Ca â†’
      Î“ âŠ¢ ğŸ™E C c' a âˆ¶ Ca â‹– c (Î´C âˆ· Î´c' âˆ· Î´a âˆ· [])

    â„•F : âˆ€ {â„“} â†’
      Î“ âŠ¢ â„•F âˆ¶ ğ’° â„“ â‹– c []
    â„•IZ :
      Î“ âŠ¢ â„•IZ âˆ¶ â„•F â‹– c []
    â„•IS : âˆ€ {n Î´n} â†’
      Î“ âŠ¢ n âˆ¶ â„•F â‹– Î´n â†’
      Î“ âŠ¢ â„•IS n âˆ¶ â„•F â‹– c (Î´n âˆ· [])
    â„•E : âˆ€ {â„“ C Î´C câ‚€ Î´câ‚€ câ‚› Î´câ‚› n Î´n Cn} â†’
      Î“ ,, â„•F {â„“ = â„“} âŠ¢ C âˆ¶ ğ’° â„“ â‹– Î´C â†’
      Î“ âŠ¢ câ‚€ âˆ¶ instantiateTerm zero â„•IZ C â‹– Î´câ‚€ â†’
      Î“ ,, â„•F {â„“ = â„“} ,, â„•F {â„“ = â„“} âŠ¢ câ‚› âˆ¶ weakenTermFrom zero
                                           (instantiateTerm (suc zero)
                                                            (â„•IS (ğ“‹ zero))
                                                            (weakenTermFrom zero C)) â‹– Î´câ‚› â†’
      Î“ âŠ¢ n âˆ¶ â„•F â‹– Î´n â†’
      instantiateTerm zero n C â‰¡ Cn â†’
      Î“ âŠ¢ â„•E C câ‚€ câ‚› n âˆ¶ Cn â‹– c (Î´C âˆ· Î´câ‚€ âˆ· Î´câ‚› âˆ· Î´n âˆ· [])
    =F : âˆ€ {â„“ A Î´A a Î´a b Î´b} â†’
      Î“ âŠ¢ A âˆ¶ ğ’° â„“ â‹– Î´A â†’ Î“ âŠ¢ a âˆ¶ A â‹– Î´a  â†’ Î“ âŠ¢ b âˆ¶ A â‹– Î´b â†’
      Î“ âŠ¢ =F A a b âˆ¶ ğ’° â„“ â‹– c (Î´A âˆ· Î´a âˆ· Î´b âˆ· [])
    =I : âˆ€ {â„“ A Î´A a Î´a} â†’
      Î“ âŠ¢ A âˆ¶ ğ’° â„“ â‹– Î´A â†’ Î“ âŠ¢ a âˆ¶ A â‹– Î´a â†’
      Î“ âŠ¢ =I a âˆ¶ =F A a a â‹– c (Î´a âˆ· [])
    =E : âˆ€ {â„“ C Î´C c' Î´c' A Î´A Î´A' a Î´a b Î´b p Î´p} â†’
        (âŠ¢A : Î“ âŠ¢ A âˆ¶ ğ’° â„“ â‹– Î´A) â†’
        (âŠ¢A' : Î“ ,, âŠ¢A âŠ¢ weakenTermFrom zero A âˆ¶ ğ’° â„“ â‹– Î´A') â†’
        (âŠ¢p : Î“ ,, âŠ¢A ,, âŠ¢A' âŠ¢ =F (weakenTermFrom zero (weakenTermFrom zero A)) ((ğ“‹ (suc zero))) ((ğ“‹ zero)) âˆ¶ ğ’° â„“ â‹– Î´p) â†’
        (âŠ¢C : Î“ ,, âŠ¢A ,, âŠ¢A' ,, âŠ¢p âŠ¢ C âˆ¶ ğ’° â„“ â‹– Î´C) â†’
        Î“ ,, âŠ¢A âŠ¢ c' âˆ¶ instantiateTerm (suc zero) (ğ“‹ zero)
                         (instantiateTerm (suc zero) (ğ“‹ zero)
                                        (instantiateTerm (suc zero) (=I (ğ“‹ zero))
                                          (weakenTermFrom zero C))) â†’
        Î“ âŠ¢ a âˆ¶ A â†’
        Î“ âŠ¢ b âˆ¶ A â†’
        Î“ âŠ¢ p âˆ¶ =F A a b â†’
        Î“ âŠ¢ =E C c' a b p âˆ¶ instantiateTerm zero a
                              (instantiateTerm zero (weakenTermFrom zero b)
                                (instantiateTerm zero
                                  (weakenTermFrom zero
                                    (weakenTermFrom zero p)) C)) â‹– c (Î´C âˆ· Î´c' âˆ· Î´a âˆ· Î´b âˆ· Î´p âˆ· [])

    Vble :
      âˆ€ {n A} â†’
      Î“ at n â‰¡ A â†’
      Î“ âŠ¢ ğ“‹ n âˆ¶ A â‹– c []

  module Test where

    0=0 : [] âŠ¢ =I â„•IZ âˆ¶ =F â„•F â„•IZ â„•IZ
    0=0 = c (c [] âˆ· []) , =I {â„“ = zero} â„•F â„•IZ


    2+2=4 : [] âŠ¢ =I (â„•IS (â„•IS (â„•IS (â„•IS â„•IZ)))) âˆ¶ =F â„•F (Î E (Î I (â„•E (Î F â„•F â„•F) (Î I (ğ“‹ zero)) (Î I (â„•IS (Î E (ğ“‹ (suc zero)) (ğ“‹ zero)))) (ğ“‹ zero))) (â„•IS (â„•IS â„•IZ))) (â„•IS (â„•IS (â„•IS (â„•IS â„•IZ))))
    2+2=4 = {!!} , {!!}

    test' : [] âŠ¢ Î I (ğ“‹ zero) âˆ¶ Î F ğŸ™F ğŸ™F â‹– c (c [] âˆ· [])
    test' = Î I (ğŸ™F {â„“ = zero}) (Vble refl)

    test'' : âˆƒ Î» N â†’ âˆƒ Î» c' â†’ âˆƒ Î» p â†’ [] âŠ¢ p âˆ¶ Î F ğŸ™F ğŸ™F â‹– c {N} c'
    test'' = 1 , c [] âˆ· [] , Î I (ğ“‹ zero) , Î I (ğŸ™F {â„“ = zero}) (Vble {1} {c (c [] âˆ· c [] âˆ· [])} refl)



  consistent : âˆ€ â„“ â†’ [] âŠ¢ ğŸ˜F âˆ¶ ğ’° â„“ Ã— Â¬ ([] âŠ¨ ğŸ˜F)
  consistent = {!!}
{-
  consistent : âˆƒ Î» bottom â†’ âˆƒ Î» â„“ â†’ [] âŠ¨ bottom âˆ¶ ğ’° â„“ Ã— Â¬ ([] âŠ¨ bottom)
  consistent = {!!}
-}

  TC-decidable : âˆ€ {N Ï‡} (Î“ : N ctxâ‹– Ï‡) (a : Term N) (A : Term N) â†’ Dec (Î“ âŠ¢ a âˆ¶ A)
  TC-decidable = {!!}

  Ïƒ-decidable : âˆ€ {N Î´} (Î“ : N ctxâ‹– Î´) (A : Term N) (â„“ : Universe)
              â†’ Î“ âŠ¢ A âˆ¶ ğ’° â„“
              â†’ âˆ€ Ïƒ
              â†’ Dec (Î“ âŠ¨ A â‰¼ Ïƒ)
  Ïƒ-decidable Î“ (ğ’° zero) â„“ x zero = yes (ğŸ™F , _ , diff zero refl , ğŸ™F)
  Ïƒ-decidable Î“ (ğ’° (suc xâ‚)) â„“ x zero = yes ({!!} , {!!} , {!!} , {!!})
  Ïƒ-decidable Î“ (ğ“‹ xâ‚) â„“ x zero = {!!}
  Ïƒ-decidable Î“ (Î F A Aâ‚) â„“ x zero = {!!}
  Ïƒ-decidable Î“ (Î I A) â„“ x zero = {!!}
  Ïƒ-decidable Î“ (Î E A Aâ‚) â„“ x zero = {!!}
  Ïƒ-decidable Î“ (Î£F A Aâ‚) â„“ x zero = {!!}
  Ïƒ-decidable Î“ (Î£I A Aâ‚) â„“ x zero = {!!}
  Ïƒ-decidable Î“ (Î£E A Aâ‚ Aâ‚‚) â„“ x zero = {!!}
  Ïƒ-decidable Î“ (+F A Aâ‚) â„“ x zero = {!!}
  Ïƒ-decidable Î“ (+IL A) â„“ x zero = {!!}
  Ïƒ-decidable Î“ (+IR A) â„“ x zero = {!!}
  Ïƒ-decidable Î“ (+E A Aâ‚ Aâ‚‚ Aâ‚ƒ) .(suc _) (.(c (_ âˆ· [])) , ğ’°C sndâ‚) zero = {!!}
  Ïƒ-decidable Î“ (+E A Aâ‚ Aâ‚‚ Aâ‚ƒ) â„“ (.(c (_ âˆ· _ âˆ· _ âˆ· _ âˆ· [])) , +E sndâ‚ sndâ‚‚ sndâ‚ƒ sndâ‚„ sndâ‚… sndâ‚† sndâ‚‡ x) zero = {!!}
  Ïƒ-decidable Î“ ğŸ˜F â„“ x zero = {!!}
  Ïƒ-decidable Î“ (ğŸ˜E A Aâ‚) â„“ x zero = {!!}
  Ïƒ-decidable Î“ ğŸ™F â„“ x zero = {!!}
  Ïƒ-decidable Î“ ğŸ™I â„“ x zero = {!!}
  Ïƒ-decidable Î“ (ğŸ™E A Aâ‚ Aâ‚‚) â„“ x zero = {!!}
  Ïƒ-decidable Î“ â„•F â„“ x zero = {!!}
  Ïƒ-decidable Î“ â„•IZ â„“ x zero = {!!}
  Ïƒ-decidable Î“ (â„•IS A) â„“ x zero = {!!}
  Ïƒ-decidable Î“ (â„•E A Aâ‚ Aâ‚‚ Aâ‚ƒ) â„“ x zero = {!!}
  Ïƒ-decidable Î“ (=F A Aâ‚ Aâ‚‚) â„“ x zero = {!!}
  Ïƒ-decidable Î“ (=I A) â„“ x zero = {!!}
  Ïƒ-decidable Î“ (=E A Aâ‚ Aâ‚‚ Aâ‚ƒ Aâ‚„) â„“ x zero = {!!}
  Ïƒ-decidable Î“ A â„“ x (suc Ïƒ) = {!!}
```
